# baseURI: https://linked.data.gov.au/def/project
# imports: http://purl.org/dc/terms/
# imports: http://www.w3.org/2004/02/skos/core
# imports: http://www.w3.org/ns/prov
# prefix: proj

@prefix dcterms: <http://purl.org/dc/terms/> .
@prefix owl: <http://www.w3.org/2002/07/owl#> .
@prefix prof: <http://www.w3.org/ns/dx/prof/> .
@prefix proj: <https://linked.data.gov.au/def/project#> .
@prefix proji: <https://linked.data.gov.au/def/project/> .
@prefix prov: <http://www.w3.org/ns/prov#> .
@prefix rdf: <http://www.w3.org/1999/02/22-rdf-syntax-ns#> .
@prefix rdfs: <http://www.w3.org/2000/01/rdf-schema#> .
@prefix sdo: <https://schema.org/> .
@prefix skos: <http://www.w3.org/2004/02/skos/core#> .
@prefix xsd: <http://www.w3.org/2001/XMLSchema#> .

<https://linked.data.gov.au/def/project/Funder>
  a prov:Role ;
  rdfs:label "funding-agent role" ;
  skos:broader <https://linked.data.gov.au/def/project/Sponsor> ;
.
<https://linked.data.gov.au/def/project/Leader>
  a prov:Role ;
  rdfs:label "activity-leader role" ;
  skos:broader <https://linked.data.gov.au/def/project/Participant> ;
  skos:narrower <https://linked.data.gov.au/def/project/PrincipalInvestigator> ;
.
<https://linked.data.gov.au/def/project/Participant>
  a prov:Role ;
  rdfs:label "activity-participant role" ;
.
<https://linked.data.gov.au/def/project/PrincipalInvestigator>
  a prov:Role ;
  rdfs:label "principal-investigator role" ;
  skos:broader <https://linked.data.gov.au/def/project/Leader> ;
.
<https://linked.data.gov.au/def/project/Sponsor>
  a prov:Role ;
  rdfs:label "project-sponsor role" ;
  skos:narrower <https://linked.data.gov.au/def/project/Funder> ;
.
<https://linked.data.gov.au/def/project/SubActivity>
  a prov:Role ;
  rdfs:label "sub-activity" ;
.
prov:Role
  rdfs:subClassOf skos:Concept ;
.
prov:agent
  dcterms:description "Link to the agent which provided the funds." ;
  skos:scopeNote "When used in the context of the sub-class proj:FundingAssociation, the value of prov:agent should identify the agent which provided the funds." ;
.
<https://linked.data.gov.au/def/project>
  a owl:Ontology ;
  a prof:Profile ;
  dcterms:contributor "Peter Brenton, CSIRO" ;
  dcterms:created "2017-08-14"^^xsd:date ;
  dcterms:creator <https://orcid.org/0000-0002-3884-3420> ;
  dcterms:description """
The PROJECT ontology is designed to enable publication of information describing projects, including research projects. It is not designed to support project management, though sub-activities are included. As far as possible PROJECT is intended to be domain-neutral, and it is expected that domains and applications will specialize or extend this ontology for more specific purposes.

The ontology gives terms to support the representation of:

- project planning, funding, goals
- project stakeholders and relationships
- project activities and timeline

One specialization is included - the **Research Project** - which has been the subject of several predecessor designs that have informed the design of this ontology, including:

- In [FOAF](http://xmlns.com/foaf/0.1/) the foaf:Project class is a stub (no specific properties) which was included primarily to act as the topic of a homepage
- [Description of a Project ontology (DOAP)](https://en.wikipedia.org/wiki/DOAP) is oriented to software development projects
- [Funding, Research Administration and Projects Ontology (FRAPO)](http://purl.org/cerif/frapo) is aimed at describing administrative information relating to grant funding and research projects. 
- [Project Documents Ontology (PDO)](http://vocab.deri.ie/pdo) relates to  various documents in a project-specific setting, like meeting minutes, status reports etc
- In [VIVO-ISF](https://github.com/openrif/vivo-isf-ontology) the [vivo:Project](http://vivoweb.org/ontology/core#Project) class is very lightweight, characterised only by its timing and geographic focus

The [DBPedia ontology](http://dbpedia.org/ontology/) provides what is probably the most general purpose class for projects: [dbo:Project](http://dbpedia.org/ontology/Project) is described as \"a temporary endeavor undertaken to achieve defined objectives\" and has key properties relating to timing, objectives, and classification (keywords).

PROJECT extends the W3C PROV-O ontology. Otherwise, it has no dependencies except for the normal RDF/OWL infrastructure ([RDF](https://www.w3.org/TR/rdf11-concepts/), [RDFS](https://www.w3.org/TR/rdf-schema/), [OWL2](https://www.w3.org/TR/owl2-quick-reference/)), [Dublin Core](http://dublincore.org/documents/2010/10/11/dcmi-terms/) for some ontology metadata, and [SKOS](https://www.w3.org/TR/skos-reference/) to support some relationships between Role values, and project classification.

A summary of the main classes and relationships in PROJECT is shown in the diagram below, including the key superclass `prov:Activity`.

![summary of PROJECT ontology](../images/Project-overview.png) 

Core classes from PROJECT vocabulary. 
""" ;
  dcterms:license <https://creativecommons.org/licenses/by/4.0/> ;
  dcterms:modified "2022-04-26"^^xsd:date ;
  dcterms:title "A Project ontology" ;
  owl:imports dcterms: ;
  owl:imports <http://www.w3.org/2004/02/skos/core> ;
  owl:imports <http://www.w3.org/ns/prov> ;
  skos:changeNote "2022-04-26 - changed namespaces to https" ;
  prof:hasResource [
      a prof:ResourceDescriptor ;
      prof:hasArtifact <https://dr-shorthair.github.io/project-ont/docs/> ;
      prof:hasRole <http://www.w3.org/ns/dx/prof/role/specification> ;
    ] ;
  prof:hasResource [
      a prof:ResourceDescriptor ;
      prof:hasArtifact <https://github.com/dr-shorthair/project-ont/blob/gh-pages/rdf/FeralCapeYork.ttl> ;
      prof:hasRole <http://www.w3.org/ns/dx/prof/role/example> ;
    ] ;
  prof:hasResource [
      a prof:ResourceDescriptor ;
      prof:hasArtifact <https://github.com/dr-shorthair/project-ont/blob/gh-pages/rdf/LevelCrossing.ttl> ;
      prof:hasRole <http://www.w3.org/ns/dx/prof/role/example> ;
    ] ;
  prof:hasResource [
      a prof:ResourceDescriptor ;
      prof:hasArtifact <https://raw.githack.com/dr-shorthair/project-ont/gh-pages/rdf/project.ttl> ;
      prof:hasRole <http://www.w3.org/ns/dx/prof/role/schema> ;
    ] ;
  prof:isProfileOf <http://www.w3.org/ns/prov-o> ;
  sdo:codeRepository <https://github.com/dr-shorthair/project-ont> ;
.
proj:FundingAssociation
  a owl:Class ;
  dcterms:description """
Association to a funder and a sum of money

![Project funding association](../images/Project-funding.png)

""" ;
  rdfs:label "Funding association" ;
  rdfs:subClassOf prov:Association ;
  rdfs:subClassOf [
      a owl:Restriction ;
      owl:cardinality "1"^^xsd:nonNegativeInteger ;
      owl:onProperty prov:agent ;
    ] ;
  rdfs:subClassOf [
      a owl:Restriction ;
      owl:hasValue <https://linked.data.gov.au/def/project/Funder> ;
      owl:onProperty prov:hadRole ;
    ] ;
  rdfs:subClassOf [
      a owl:Restriction ;
      owl:minCardinality "1"^^xsd:nonNegativeInteger ;
      owl:onProperty proj:fundsProvided ;
    ] ;
  skos:example """
ex:FA3
  rdf:type proj:FundingAssociation ;
  rdfs:label \"Level crossing removal project phase 1 funding arrangement\" ;
  rdfs:seeAlso <http://www.premier.vic.gov.au/contract-awarded-for-first-four-level-crossing-removals/> ;
  proj:fundsProvided [
    rdf:type proj:SumOfMoney ;
    proj:moneyAmount \"524000000\"^^xsd:decimal ;
    proj:moneyCurrency <https://dbpedia.org/resource/Australian_dollar> ;
  ] ;
  prov:agent <http://www.vic.gov.au/> ;
 .
""" ;
.
proj:Project
  a owl:Class ;
  dcterms:description """
A Project is a planned activity with a budget, a sponsor, and a leader.

Project stakeholders are indicated using `prov:wasAssociatedWith` or the `prov:qualifiedAssociation` structure which allows their role to be catpured. Some special stakeholders have specific sub-properties with the roles fixed, including project-leader, project-participant, and project-funder.

Activities within a project are indicated using the `proj:hasSubActivity` (simple) or `proj:subActivityAssociation` properties - the latter allowing the nature of the relationshp to be described as well. 

![Project details](../images/Project.png)

""" ;
  rdfs:label "Project" ;
  rdfs:subClassOf prov:Activity ;
  rdfs:subClassOf [
      a owl:Restriction ;
      owl:cardinality "1"^^xsd:nonNegativeInteger ;
      owl:onProperty proj:hadBudgetTotal ;
    ] ;
  rdfs:subClassOf [
      a owl:Restriction ;
      owl:cardinality "1"^^xsd:nonNegativeInteger ;
      owl:onProperty proj:plannedEnd ;
    ] ;
  rdfs:subClassOf [
      a owl:Restriction ;
      owl:cardinality "1"^^xsd:nonNegativeInteger ;
      owl:onProperty proj:plannedStart ;
    ] ;
  rdfs:subClassOf [
      a owl:Restriction ;
      owl:minCardinality "1"^^xsd:nonNegativeInteger ;
      owl:onProperty proj:hadLeader ;
    ] ;
  rdfs:subClassOf [
      a owl:Restriction ;
      owl:minCardinality "1"^^xsd:nonNegativeInteger ;
      owl:onProperty proj:hadPlan ;
    ] ;
  rdfs:subClassOf [
      a owl:Restriction ;
      owl:minCardinality "1"^^xsd:nonNegativeInteger ;
      owl:onProperty proj:hadSponsor ;
    ] ;
  skos:example """
ex:Project1
rdf:type proj:Project ;
rdfs:label \"Victoria level-crossing removal - phase 1\" ;
proj:hadBudgetTotal [
  rdf:type proj:SumOfMoney ;
  rdfs:label \"Level crossing removal phase 1 budget\" ;
  proj:moneyAmount \"524000000\"^^xsd:decimal ;
  proj:moneyCurrency <https://dbpedia.org/resource/Australian_dollar> ;
] ;
proj:hadLeader ex:johnholland-kbr ;
proj:hadSponsor <http://levelcrossings.vic.gov.au/about/about-the-authority> ;
proj:hadSubActivity ex:BentleighLevelCrossingRemoval ;
proj:hadSubActivity ex:BurkeRoadLevelCrossingRemoval ;
proj:hadSubActivity ex:McKinnonRoadLevelCrossingRemoval ;
proj:hadSubActivity ex:NorthRoadLevelCrossingRemoval ;
proj:wasFundedThrough [
  rdf:type proj:FundingAssociation ;
  rdfs:label \"Level crossing removal project phase 1 funding arrangement\" ;
  rdfs:seeAlso <http://www.premier.vic.gov.au/contract-awarded-for-first-four-level-crossing-removals/> ;
  proj:fundsProvided [
    rdf:type proj:SumOfMoney ;
    proj:moneyAmount \"524000000\"^^xsd:decimal ;
    proj:moneyCurrency <https://dbpedia.org/resource/Australian_dollar> ;
  ] ;
  prov:agent <http://www.vic.gov.au/> ;
] ;
rdfs:label \"Victoria level-crossing removal - phase 1\" ;
proj:plannedEnd \"2017-03-31\"^^xsd:date ;
proj:plannedStart \"2015-10-01\"^^xsd:date ;
prov:atLocation <https://dbpedia.org/resource/Melbourne> ;
prov:endedAtTime \"2016-10-31T00:00:00\"^^xsd:dateTime ;
prov:startedAtTime \"2015-10-01T00:00:00\"^^xsd:dateTime ;
.
""" ;
.
proj:ResearchProject
  a owl:Class ;
  dcterms:description """
A research project is a project that has 

- one or more PIs who are individual persons, and 
- should be classified according to standard research classification, such as the Australian Bureau of Statistics ANZSRC-FOR or NASA's Global Change Master Directory - Science Keywords. 
""" ;
  rdfs:label "Research Project" ;
  rdfs:subClassOf proj:Project ;
  rdfs:subClassOf [
      a owl:Restriction ;
      owl:minCardinality "1"^^xsd:nonNegativeInteger ;
      owl:onProperty proj:hadFieldOfResearch ;
    ] ;
  skos:example """
ex:Project2
rdf:type proj:Project ;
rdf:type proj:ResearchProject ;
rdfs:label \"Improved management of feral animals in remote tropical Australia\" ;
proj:budgetTotal [
  rdf:type proj:SumOfMoney ;
  proj:moneyAmount 0 ;
  proj:moneyCurrency <https://dbpedia.org/resource/Australian_dollar> ;
] ;
proj:hadFieldOfResearch <http://purl.org/au-research/vocabulary/anzsrc-for/2008/050202> ;
proj:hadPrincipalInvestigator <http://orcid.org/0000-0002-5823-7364> ;
proj:hadSponsor <http://dbpedia.org/resource/Commonwealth_Scientific_and_Industrial_Research_Organisation> ;
proj:hadSubActivity ex:Aerial ;
proj:wasSubActivityOf <http://www.environment.gov.au/science/nesp> ;
rdfs:label \"Improved management of feral animals in remote tropical Australia\" ;
proj:hadObjective \"To develop a robust understanding of the costs and benefits of selected feral animal control programs on reducing impacts to natural and cultural values.\" ;
proj:plannedEnd \"2022-12-31\"^^xsd:date ;
proj:plannedStart \"2012-12-31\"^^xsd:date ;
proj:projectParticipant <mailto:peter.brenton@csiro.au> ;
proj:hadPlan ex:FCY-project-plan ;
proj:wasFundedThrough [
  rdf:type proj:FundingAssociation ;
  proj:fundsProvided [
    rdf:type proj:SumOfMoney ;
    proj:moneyAmount 0 ;
    proj:moneyCurrency <https://dbpedia.org/resource/Australian_dollar> ;
  ] ;
  prov:agent <http://dbpedia.org/resource/Government_of_Australia> ;
] ;
prov:atLocation <http://dbpedia.org/resource/Archer_River,_Queensland> ;
prov:generated <https://doi.org/10.1071/WF15133> ;
prov:startedAtTime \"2012-12-31T00:00:00\"^^xsd:dateTime ;
.
""" ;
.
proj:SumOfMoney
  a owl:Class ;
  dcterms:description "A sum of money, expressed as an amount and a specified currency" ;
  rdfs:label "Sum of money" ;
  rdfs:subClassOf owl:Thing ;
  rdfs:subClassOf [
      a owl:Restriction ;
      owl:cardinality "1"^^xsd:nonNegativeInteger ;
      owl:onProperty proj:moneyAmount ;
    ] ;
  rdfs:subClassOf [
      a owl:Restriction ;
      owl:cardinality "1"^^xsd:nonNegativeInteger ;
      owl:onProperty proj:moneyCurrency ;
    ] ;
  skos:example """
ex:SM4
    rdf:type proj:SumOfMoney ;
    proj:moneyAmount \"524000000\"^^xsd:decimal ; 
    proj:moneyCurrency <https://dbpedia.org/resource/Australian_dollar> ;
 .
""" ;
.
proj:fundingScheme
  a owl:AnnotationProperty ;
  a owl:ObjectProperty ;
  dcterms:description """
Link to description of funding scheme, e.g.

- [European Commission Horizon 2020](https://ec.europa.eu/programmes/horizon2020/)
- [Australian National Collaborative Research Infrastructure Strategy](https://www.education.gov.au/national-collaborative-research-infrastructure-strategy-ncris)
""" ;
  rdfs:domain proj:FundingAssociation ;
  rdfs:label "pointer to funding-scheme" ;
.
proj:fundsProvided
  a owl:ObjectProperty ;
  dcterms:description "Link to a sum of money." ;
  rdfs:label "funding provided" ;
  rdfs:range proj:SumOfMoney ;
.
proj:grantNumber
  a owl:AnnotationProperty ;
  a owl:DatatypeProperty ;
  dcterms:description "The grant or contract number assigned to the funding arrangement by the funder.  'Grant number' is common for research or charitable projects, 'Contract number' in a commercial context." ;
  rdfs:domain proj:FundingAssociation ;
  rdfs:label "grant or contract number" ;
  rdfs:range xsd:string ;
.
proj:hadAreaOfInterest
  a owl:AnnotationProperty ;
  a owl:ObjectProperty ;
  dcterms:description """
Address, place, locality, location, etc
""" ;
  rdfs:domain proj:Project ;
  rdfs:label "has area of interest" ;
  rdfs:range dcterms:Location ;
  rdfs:subPropertyOf prov:atLocation ;
  skos:editorialNote """
The name and label of this property are phrased retrospectively (had, was) which is consistent with PROV-O, but may be used for a contemporary relationship (has, is) while the project is underway.
""" ;
.
proj:hadBudgetTotal
  a owl:ObjectProperty ;
  dcterms:description """
Basic funding arrangements are captured through the `proj:hadSponsor` and `proj:hadBudgetTotal` properties.
  
More complex arrangements, for example if multiple funders are involved, can be captured through the `proj:wasFundedThrough` property, which links a funding agent with a funding amount in the context of a project.
""" ;
  rdfs:domain proj:Project ;
  rdfs:label "total project budget" ;
  rdfs:range proj:SumOfMoney ;
  skos:editorialNote """
The name and label of this property are phrased retrospectively (had, was) which is consistent with PROV-O, but may be used for a contemporary relationship (has, is) while the project is underway.
""" ;
.
proj:hadFieldOfResearch
  a owl:AnnotationProperty ;
  a owl:ObjectProperty ;
  dcterms:description """
The field of research of the research project.
""" ;
  rdfs:domain proj:ResearchProject ;
  rdfs:label "field of research" ;
  rdfs:range skos:Concept ;
  rdfs:subPropertyOf dcterms:subject ;
  skos:editorialNote """
The name and label of this property are phrased retrospectively (had, was) which is consistent with PROV-O, but may be used for a contemporary relationship (has, is) while the project is underway.
""" ;
  skos:scopeNote "The value is usually taken from a curated vocabulary, such as [ANZSRC Fields of Research](http://www.abs.gov.au/ausstats/abs@.nsf/0/6BB427AB9696C225CA2574180004463E), [Re3data subjects](http://www.re3data.org/browse/by-subject/), [EDAM Topic](http://edamontology.org/topic_0003) or [Scigraph subjects](https://github.com/springernature/scigraph/wiki)" ;
.
proj:hadLeader
  a owl:ObjectProperty ;
  dcterms:description """
There are a number of distinctive stakeholders in a project, in particular: a leader who is accountable for the delivery of project outcomes; a sponsor under whose authority the project is undertaken; funders; and project staff or participants.
In some cases it is useful to provide specific details of a participant's role in the project.
PROJECT provides a number of ways to represent the relationships of stakeholders to projects and activities.

The standard role of _leader_ is implemented as a directly named property from an `prov:Activity` to a `prov:Agent`, and _sponsor_ as a directly named property from a `proj:Project` to a `prov:Agent`.

We distinguish one sub-class, the `proj:ResearchProject`, in which the leader(s) is known as a _Principal Investigator_, and which is classified according to its _field of research_.

""" ;
  rdfs:label "leader" ;
  rdfs:range prov:Person ;
  rdfs:subPropertyOf prov:wasAssociatedWith ;
  skos:editorialNote """
Equivalent to property-chain prov:qualifiedAssociation-prov:agent with the value of 'role' on the intermediate prov:Association being set to proji:Leader
which might be axiomatized as 

  owl:propertyChainAxiom (
      [
        rdf:type owl:ObjectProperty ;
        rdfs:range [
            rdf:type owl:Class ;
            rdfs:subClassOf prov:Association ;
            rdfs:subClassOf [
                rdf:type owl:Restriction ;
                owl:hasValue proji:Leader ;
                owl:onProperty prov:hadRole ;
              ] ;
          ] ;
        rdfs:subPropertyOf prov:qualifiedAssociation ;
      ]
      prov:agent
    ) ;
""" ;
  skos:editorialNote """
The name and label of this property are phrased retrospectively (had, was) which is consistent with PROV-O, but may be used for a contemporary relationship (has, is) while the project is underway.
""" ;
.
proj:hadObjective
  a owl:AnnotationProperty ;
  a owl:DatatypeProperty ;
  dcterms:description "Textual description of project objective." ;
  rdfs:domain proj:Project ;
  rdfs:label "project objective" ;
.
proj:hadPlan
  a owl:ObjectProperty ;
  dcterms:description "The project plan." ;
  rdfs:domain proj:Project ;
  rdfs:label "Project plan" ;
  rdfs:range prov:Plan ;
  rdfs:subPropertyOf prov:used ;
  skos:editorialNote "A new property is required to associated a plan with a project activity because the domain of `prov:hadPlan` is `prov:Association`." ;
.
proj:hadPrincipalInvestigator
  a owl:ObjectProperty ;
  dcterms:description """
The person who acts as principal investigator on the research project.
""" ;
  rdfs:domain proj:ResearchProject ;
  rdfs:label "principal investigator" ;
  rdfs:subPropertyOf proj:hadLeader ;
  skos:editorialNote """
The name and label of this property are phrased retrospectively (had, was) which is consistent with PROV-O, but may be used for a contemporary relationship (has, is) while the project is underway.
""" ;
.
proj:hadRelatedActivity
  a owl:ObjectProperty ;
  dcterms:description """
Link from an activity to a related activity.
""" ;
  rdfs:domain prov:Activity ;
  rdfs:label "had related activity" ;
  rdfs:range prov:ActivityInfluence ;
  rdfs:subPropertyOf prov:qualifiedInfluence ;
  owl:inverseOf prov:activity ;
  skos:editorialNote """
The name and label of this property are phrased retrospectively (had, was) which is consistent with PROV-O, but may be used for a contemporary relationship (has, is) while the project is underway.
""" ;
  skos:editorialNote """
This is more general than `prov:qualifiedCommunication` since it is not predicated on the exchange of an entity. 
""" ;
.
proj:hadSponsor
  a owl:ObjectProperty ;
  dcterms:description """
There are a number of distinctive stakeholders in a project, in particular: a leader who is accountable for the delivery of project outcomes; a sponsor under whose authority the project is undertaken; funders; and project staff or participants.
In some cases it is useful to provide specific details of a participant's role in the project.
PROJECT provides a number of ways to represent the relationships of stakeholders to projects and activities.

Basic funding arrangements are captured through the `proj:hadSponsor` and `proj:hadBudgetTotal` properties.
More complex arrangements, for example if multiple funders are involved, can be captured through the `proj:wasFundedThrough` property, which links a funding agent with a funding amount in the context of a project.

![Project funding association](../images/Project-funding.png)

""" ;
  rdfs:domain proj:Project ;
  rdfs:label "activity sponsor" ;
  rdfs:subPropertyOf prov:wasAssociatedWith ;
  skos:editorialNote """
Equivalent to property-chain prov:qualifiedAssociation-prov:agent with the value of 'role' on the intermediate prov:Association being set to proji:Sponsor
which might be axiomatized as 

  owl:propertyChainAxiom (
      [
        rdf:type owl:ObjectProperty ;
        rdfs:range [
            rdf:type owl:Class ;
            rdfs:subClassOf prov:Association ;
            rdfs:subClassOf [
                rdf:type owl:Restriction ;
                owl:hasValue proji:Sponsor ;
                owl:onProperty prov:hadRole ;
              ] ;
          ] ;
        rdfs:subPropertyOf prov:qualifiedAssociation ;
      ]
      prov:agent
    ) ;
""" ;
  skos:editorialNote """
The name and label of this property are phrased retrospectively (had, was) which is consistent with PROV-O, but may be used for a contemporary relationship (has, is) while the project is underway.
""" ;
.
proj:hadSubActivity
  a owl:ObjectProperty ;
  dcterms:description """
Relationship from an activity to a subsidiary activity.
""" ;
  rdfs:domain prov:Activity ;
  rdfs:label "has sub-activity" ;
  rdfs:range prov:Activity ;
  skos:editorialNote """
The name and label of this property are phrased retrospectively (had, was) which is consistent with PROV-O, but may be used for a contemporary relationship (has, is) while the project is underway.
""" ;
  skos:editorialNote "This property is more general than prov:wasInformedBy since it is not predicated on the exchange of an entity. " ;
.
proj:moneyAmount
  a owl:DatatypeProperty ;
  dcterms:description "Numeric value of a sum of money, which must be scaled by a specified currency to get the actual value" ;
  rdfs:domain proj:SumOfMoney ;
  rdfs:label "Money amount" ;
  rdfs:range xsd:decimal ;
.
proj:moneyCurrency
  a owl:ObjectProperty ;
  rdfs:domain proj:SumOfMoney ;
  rdfs:label "currency of a sum of money" ;
.
proj:plannedEnd
  a owl:DatatypeProperty ;
  dcterms:description "The date and time at which an activity was planned to end. See also project:plannedStart."@en ;
  rdfs:label "planned end-date|time" ;
  skos:scopeNote "Usually an xsd:date or xsd:dateTime" ;
.
proj:plannedStart
  a owl:DatatypeProperty ;
  dcterms:description "The date and time at which an activity was planned to start. See also project:plannedEnd."@en ;
  rdfs:label "planned start-date|time" ;
  skos:scopeNote "Usually an xsd:date or xsd:dateTime" ;
.
proj:wasFundedThrough
  a owl:ObjectProperty ;
  dcterms:description """
Basic funding arrangements are captured through the `proj:hadSponsor` and `proj:hadBudgetTotal` properties.
More complex arrangements, for example if multiple funders are involved, can be captured through the `proj:wasFundedThrough` property, which links a funding agent with a funding amount in the context of a project.

![Project funding association](../images/Project-funding.png)

""" ;
  rdfs:domain proj:Project ;
  rdfs:label "had funding association" ;
  rdfs:range proj:FundingAssociation ;
  skos:editorialNote """
Sub-property of prov:qualifiedAssociation with the value of 'role' on the intermediate prov:Association being set to proji:Sponsor
which might be axiomatized as 

  rdfs:subPropertyOf [
      rdf:type owl:ObjectProperty ;
      rdfs:range [
          rdf:type owl:Class ;
          rdfs:subClassOf prov:Association ;
          rdfs:subClassOf [
              rdf:type owl:Restriction ;
              owl:hasValue proji:Sponsor ;
              owl:onProperty prov:hadRole ;
            ] ;
        ] ;
      rdfs:subPropertyOf prov:qualifiedAssociation ;
    ] ;
""" ;
  skos:editorialNote """
The name and label of this property are phrased retrospectively (had, was) which is consistent with PROV-O, but may be used for a contemporary relationship (has, is) while the project is underway.
""" ;
.
proj:wasSubActivityOf
  a owl:ObjectProperty ;
  dcterms:description """
Relationship from an activity to its parent activity or project.
""" ;
  rdfs:label "is sub-activity of" ;
  rdfs:subPropertyOf prov:wasInformedBy ;
  owl:inverseOf proj:hadSubActivity ;
  skos:editorialNote """
The name and label of this property are phrased retrospectively (had, was) which is consistent with PROV-O, but may be used for a contemporary relationship (has, is) while the project is underway.
""" ;
.
<https://linked.data.gov.au/org/csiro>
  a sdo:Organization ;
  sdo:name "Commonwealth Scientific and Industrial Research Organisation" ;
  sdo:url <https://csiro.au> ;
.
<https://orcid.org/0000-0002-3884-3420>
  a sdo:Person ;
  sdo:affiliation <https://linked.data.gov.au/org/csiro> ;
  sdo:email "simon.cox@csiro.au" ;
  sdo:identifier "https://orcid.org/0000-0002-3884-3420"^^xsd:anyURI ;
  sdo:name "Simon J D Cox" ;
  sdo:subjectOf <https://people.csiro.au/C/S/simon-cox> ;
.
<https://people.csiro.au/C/S/simon-cox>
  a sdo:AboutPage ;
.
